extraction/theories/ESubstitution.v
@@ -14,7 +14,6 @@ Existing Instance config.default_checker_flags.
 Module PA := PCUICAst.
 Module P := PCUICWcbvEval.
 
-
 Inductive free : nat -> term -> Prop :=
 | free_tRel x : free x (tRel x)
 | free_tApp1 x s t : free x s -> free x (tApp s t)
@@ -26,10 +25,10 @@ Inductive free : nat -> term -> Prop :=
 | free_tCase1 x p s brs : free x s -> free x (tCase p s brs)
 | free_tCase2 x p s brs n b : free x b -> In (n, b) brs -> free x (tCase p s brs).
 
-
 Lemma subst_free_ext sigma tau t :
-  (forall x, free x t -> nth_error sigma x = nth_error tau x) -> subst sigma 0 t = subst tau 0 t.
+  (forall n, free n t -> nth_error sigma n = nth_error tau n) -> subst sigma 0 t = subst tau 0 t.
 Admitted.
+
 
 
 
